code/nist-pcurves/Hacl.Impl.PCurves.Field.fsti
@@ -20,7 +20,7 @@ module CC = Hacl.Impl.PCurves.Constants
 
 
 inline_for_extraction noextract
-let bn_is_lt_prime_mask_t  {| S.curve_params |} {| CC.curve_constants |} {| bn:bn_ops |} =
+let bn_is_lt_prime_mask_t  {| S.curve_params |} {| bn:bn_ops |} {| CC.curve_constants |} =
     f:felem -> Stack uint64
   (requires fun h -> live h f)
   (ensures  fun h0 r h1 -> modifies0 h0 h1 /\
@@ -28,7 +28,7 @@ let bn_is_lt_prime_mask_t  {| S.curve_params |} {| CC.curve_constants |} {| bn:b
 
 [@(strict_on_arguments [0;1;2])]
 inline_for_extraction noextract
-val bn_is_lt_prime_mask_g {| S.curve_params |} {| CC.curve_constants |} {| bn:bn_ops |}: bn_is_lt_prime_mask_t
+val bn_is_lt_prime_mask_g {| S.curve_params |}  {| bn:bn_ops |} {| CC.curve_constants |}: bn_is_lt_prime_mask_t
 
 [@(strict_on_arguments [0;1])]
 inline_for_extraction noextract
@@ -44,7 +44,7 @@ val feq_mask {| S.curve_params |} {| bn:bn_ops |}:
 ///  Field Arithmetic
 
 inline_for_extraction noextract
-let fadd_t {| S.curve_params |} {| CC.curve_constants |} {| bn:bn_ops |} =
+let fadd_t {| S.curve_params |}  {| bn:bn_ops |} {| CC.curve_constants |} =
   res:felem -> x:felem -> y:felem -> Stack unit
   (requires fun h ->
     live h x /\ live h y /\ live h res /\
@@ -56,22 +56,12 @@ let fadd_t {| S.curve_params |} {| CC.curve_constants |} {| bn:bn_ops |} =
 
 [@(strict_on_arguments [0;1;2])]
 inline_for_extraction noextract
-val fadd_g {| S.curve_params |} {| CC.curve_constants |} {| bn:bn_ops |}:
+val fadd_g {| S.curve_params |}  {| bn:bn_ops |} {| CC.curve_constants |}:
   fadd_t
 
-[@(strict_on_arguments [0;1;2])]
-inline_for_extraction noextract
-val fdouble {| S.curve_params |} {| CC.curve_constants |} {| bn:bn_ops |}:
-  res:felem -> x:felem -> Stack unit
-  (requires fun h ->
-    live h x /\ live h res /\ eq_or_disjoint x res /\
-    as_nat h x < S.prime)
-  (ensures fun h0 _ h1 -> modifies (loc res) h0 h1 /\
-    as_nat h1 res == (2 * as_nat h0 x) % S.prime /\
-    CC.fmont_as_nat h1 res == (2 * CC.fmont_as_nat h0 x) % S.prime)
 
 inline_for_extraction noextract
-let fsub_t {| S.curve_params |} {| CC.curve_constants |} {| bn:bn_ops |} =
+let fsub_t {| S.curve_params |}  {| bn:bn_ops |} {| CC.curve_constants |} =
   res:felem -> x:felem -> y:felem -> Stack unit
   (requires fun h ->
     live h res /\ live h x /\ live h y /\
@@ -83,22 +73,11 @@ let fsub_t {| S.curve_params |} {| CC.curve_constants |} {| bn:bn_ops |} =
 
 [@(strict_on_arguments [0;1;2])]
 inline_for_extraction noextract
-val fsub_g {| S.curve_params |} {| CC.curve_constants |} {| bn:bn_ops |}:
+val fsub_g {| S.curve_params |}  {| bn:bn_ops |} {| CC.curve_constants |}:
   fsub_t
 
 inline_for_extraction noextract
-let fnegate_conditional_vartime_t {| S.curve_params |} {| CC.curve_constants |} {| bn:bn_ops |} =
-  f:felem -> is_negate:bool -> Stack unit
-  (requires fun h -> live h f /\ as_nat h f < S.prime)
-  (ensures  fun h0 _ h1 -> modifies (loc f) h0 h1 /\ as_nat h1 f < S.prime /\
-    as_nat h1 f == (if is_negate then (S.prime - as_nat h0 f) % S.prime else as_nat h0 f))
-
-[@(strict_on_arguments [0;1;2])]
-inline_for_extraction noextract
-val fnegate_conditional_vartime_g {| S.curve_params |} {| CC.curve_constants |} {| bn:bn_ops |}: fnegate_conditional_vartime_t
-
-inline_for_extraction noextract
-let fmul_t {| S.curve_params |} {| CC.curve_constants |} {| bn:bn_ops |} =
+let fmul_t {| S.curve_params |}  {| bn:bn_ops |} {| CC.curve_constants |} =
   res:felem -> x:felem -> y:felem -> Stack unit
   (requires fun h ->
     live h x /\ live h y /\ live h res /\
@@ -110,11 +89,11 @@ let fmul_t {| S.curve_params |} {| CC.curve_constants |} {| bn:bn_ops |} =
 
 [@(strict_on_arguments [0;1;2])]
 inline_for_extraction noextract
-val fmul_g {| S.curve_params |} {| CC.curve_constants |} {| bn:bn_ops |}:
+val fmul_g {| S.curve_params |}  {| bn:bn_ops |} {| CC.curve_constants |}:
   fmul_t
 
 inline_for_extraction noextract
-let fsqr_t {| S.curve_params |} {| CC.curve_constants |} {| bn:bn_ops |} =
+let fsqr_t {| S.curve_params |}  {| bn:bn_ops |} {| CC.curve_constants |} =
   res:felem -> x:felem -> Stack unit
   (requires fun h ->
     live h x /\ live h res /\ eq_or_disjoint x res /\
@@ -125,11 +104,11 @@ let fsqr_t {| S.curve_params |} {| CC.curve_constants |} {| bn:bn_ops |} =
 
 [@(strict_on_arguments [0;1;2])]
 inline_for_extraction noextract
-val fsqr_g {| S.curve_params |} {| CC.curve_constants |} {| bn:bn_ops |}:
+val fsqr_g {| S.curve_params |}  {| bn:bn_ops |} {| CC.curve_constants |}:
     fsqr_t
 
 inline_for_extraction noextract
-let from_mont_t {| S.curve_params |} {| CC.curve_constants |} {| bn:bn_ops |} =
+let from_mont_t {| S.curve_params |}  {| bn:bn_ops |} {| CC.curve_constants |} =
   res:felem -> x:felem -> Stack unit
   (requires fun h ->
     live h x /\ live h res /\ as_nat h x < S.prime)
@@ -139,11 +118,11 @@ let from_mont_t {| S.curve_params |} {| CC.curve_constants |} {| bn:bn_ops |} =
 
 [@(strict_on_arguments [0;1;2])]
 inline_for_extraction noextract
-val from_mont_g {| S.curve_params |} {| CC.curve_constants |} {| bn:bn_ops |}:
+val from_mont_g {| S.curve_params |}  {| bn:bn_ops |} {| CC.curve_constants |}:
   from_mont_t
 
 inline_for_extraction noextract
-let to_mont_t {| S.curve_params |} {| CC.curve_constants |} {| bn:bn_ops |} =
+let to_mont_t {| S.curve_params |}  {| bn:bn_ops |} {| CC.curve_constants |} =
   res:felem -> f:felem -> Stack unit
   (requires fun h ->
     live h f /\ live h res /\ eq_or_disjoint f res /\
@@ -153,14 +132,49 @@ let to_mont_t {| S.curve_params |} {| CC.curve_constants |} {| bn:bn_ops |} =
 
 [@(strict_on_arguments [0;1;2])]
 inline_for_extraction noextract
-val to_mont_g {| S.curve_params |} {| CC.curve_constants |} {| bn:bn_ops |}:
+val to_mont_g {| S.curve_params |}  {| bn:bn_ops |} {| CC.curve_constants |}:
     to_mont_t
 
 ///  Special cases of the above functions
 
+
+[@(strict_on_arguments [0;1;2])]
+inline_for_extraction
+class field_ops {| S.curve_params |} {| bn:bn_ops |} {| CC.curve_constants |} = {
+  bn_is_lt_prime_mask: bn_is_lt_prime_mask_t;
+  fadd:fadd_t;
+  fsub:fsub_t;
+  fmul:fmul_t;
+  fsqr:fsqr_t;
+  from_mont: from_mont_t;
+  to_mont: to_mont_t;
+}
+
+inline_for_extraction noextract
+let fnegate_conditional_vartime_t {| S.curve_params |}  {| bn:bn_ops |} {| CC.curve_constants |} {| field_ops |} =
+  f:felem -> is_negate:bool -> Stack unit
+  (requires fun h -> live h f /\ as_nat h f < S.prime)
+  (ensures  fun h0 _ h1 -> modifies (loc f) h0 h1 /\ as_nat h1 f < S.prime /\
+    as_nat h1 f == (if is_negate then (S.prime - as_nat h0 f) % S.prime else as_nat h0 f))
+
 [@(strict_on_arguments [0;1;2])]
 inline_for_extraction noextract
-val fmul_by_b_coeff {| S.curve_params |} {| CC.curve_constants |} {| bn:bn_ops |}:
+val fnegate_conditional_vartime {| S.curve_params |}  {| bn:bn_ops |} {| CC.curve_constants |} {| field_ops |} : fnegate_conditional_vartime_t
+
+[@(strict_on_arguments [0;1;2])]
+inline_for_extraction noextract
+val fdouble {| S.curve_params |}  {| bn:bn_ops |} {| CC.curve_constants |} {| field_ops |}:
+  res:felem -> x:felem -> Stack unit
+  (requires fun h ->
+    live h x /\ live h res /\ eq_or_disjoint x res /\
+    as_nat h x < S.prime)
+  (ensures fun h0 _ h1 -> modifies (loc res) h0 h1 /\
+    as_nat h1 res == (2 * as_nat h0 x) % S.prime /\
+    CC.fmont_as_nat h1 res == (2 * CC.fmont_as_nat h0 x) % S.prime)
+
+[@(strict_on_arguments [0;1;2])]
+inline_for_extraction noextract
+val fmul_by_b_coeff {| S.curve_params |}  {| bn:bn_ops |} {| CC.curve_constants |} {| field_ops |}:
   res:felem -> x:felem -> Stack unit
   (requires fun h ->
     live h x /\ live h res /\ eq_or_disjoint x res /\
@@ -173,7 +187,7 @@ val fmul_by_b_coeff {| S.curve_params |} {| CC.curve_constants |} {| bn:bn_ops |
 
 [@(strict_on_arguments [0;1;2])]
 inline_for_extraction noextract
-val fcube {| S.curve_params |} {| CC.curve_constants |} {| bn:bn_ops |}:
+val fcube {| S.curve_params |}  {| bn:bn_ops |} {| CC.curve_constants |} {| field_ops |}:
   res:felem -> x:felem -> Stack unit
   (requires fun h ->
     live h x /\ live h res /\ disjoint x res /\
@@ -183,15 +197,4 @@ val fcube {| S.curve_params |} {| CC.curve_constants |} {| bn:bn_ops |}:
     CC.fmont_as_nat h1 res =
       S.fmul (S.fmul (CC.fmont_as_nat h0 x) (CC.fmont_as_nat h0 x)) (CC.fmont_as_nat h0 x))
 
-[@(strict_on_arguments [0;1;2])]
-inline_for_extraction
-class field_ops {| S.curve_params |} {| CC.curve_constants |} {| bn:bn_ops |} = {
-  bn_is_lt_prime_mask: bn_is_lt_prime_mask_t;
-  fadd:fadd_t;
-  fsub:fsub_t;
-  fnegate_conditional_vartime:fnegate_conditional_vartime_t;
-  fmul:fmul_t;
-  fsqr:fsqr_t;
-  from_mont: from_mont_t;
-  to_mont: to_mont_t;
-}
+
