code/nist-pcurves/Hacl.Impl.PCurves.Finv.fst
@@ -48,26 +48,26 @@ let mk_to_pcurve_prime_comm_monoid {| cp:S.curve_params |} : BE.to_comm_monoid U
 
 [@(strict_on_arguments [0;1])]
 inline_for_extraction noextract
-val one_mod {| cp:S.curve_params |} {| CC.curve_constants |} : BE.lone_st U64 cp.bn_limbs 0ul mk_to_pcurve_prime_comm_monoid
+val one_mod {| cp:S.curve_params |} {| bn_ops |} {| CC.curve_constants |} : BE.lone_st U64 cp.bn_limbs 0ul mk_to_pcurve_prime_comm_monoid
 
-let one_mod {| cp:S.curve_params |} {| cc:CC.curve_constants |} ctx one = cc.make_fone one
-
-
-[@(strict_on_arguments [0;1;2;3])]
-inline_for_extraction noextract
-val mul_mod {| cp:S.curve_params |} {| CC.curve_constants |} {| bn_ops |} {| f:field_ops |} : BE.lmul_st U64 cp.bn_limbs 0ul mk_to_pcurve_prime_comm_monoid
-let mul_mod {| cp:S.curve_params |} {| CC.curve_constants |} {| bn_ops |} {| f:field_ops |} ctx x y xy = f.fmul xy x y
+let one_mod {| cp:S.curve_params |} {| bn_ops |} {| cc:CC.curve_constants |} ctx one = cc.make_fone one
 
 
 [@(strict_on_arguments [0;1;2;3])]
 inline_for_extraction noextract
-val sqr_mod {| cp:S.curve_params |} {| CC.curve_constants |} {| bn_ops |} {| f:field_ops |} : BE.lsqr_st U64 cp.bn_limbs 0ul mk_to_pcurve_prime_comm_monoid
-let sqr_mod {| cp:S.curve_params |} {| CC.curve_constants |} {| bn_ops |} {| f:field_ops |} ctx x xx = f.fsqr xx x
+val mul_mod {| cp:S.curve_params |} {| bn_ops |} {| CC.curve_constants |}  {| f:field_ops |} : BE.lmul_st U64 cp.bn_limbs 0ul mk_to_pcurve_prime_comm_monoid
+let mul_mod {| cp:S.curve_params |} {| bn_ops |} {| CC.curve_constants |}  {| f:field_ops |} ctx x y xy = f.fmul xy x y
 
 
 [@(strict_on_arguments [0;1;2;3])]
 inline_for_extraction noextract
-let mk_pcurve_prime_concrete_ops {| cp:S.curve_params |} {| CC.curve_constants |} {| bn_ops |} {| f:field_ops |} : BE.concrete_ops U64 cp.bn_limbs 0ul = {
+val sqr_mod {| cp:S.curve_params |} {| bn_ops |} {| CC.curve_constants |}  {| f:field_ops |} : BE.lsqr_st U64 cp.bn_limbs 0ul mk_to_pcurve_prime_comm_monoid
+let sqr_mod {| cp:S.curve_params |} {| bn_ops |} {| CC.curve_constants |}  {| f:field_ops |} ctx x xx = f.fsqr xx x
+
+
+[@(strict_on_arguments [0;1;2;3])]
+inline_for_extraction noextract
+let mk_pcurve_prime_concrete_ops {| cp:S.curve_params |} {| bn_ops |} {| CC.curve_constants |}  {| f:field_ops |} : BE.concrete_ops U64 cp.bn_limbs 0ul = {
   BE.to = mk_to_pcurve_prime_comm_monoid;
   BE.lone = one_mod;
   BE.lmul = mul_mod;
@@ -77,14 +77,14 @@ let mk_pcurve_prime_concrete_ops {| cp:S.curve_params |} {| CC.curve_constants |
 
 [@(strict_on_arguments [0;1;2;3])]
 inline_for_extraction noextract
-val fsquare_times_in_place {| cp:S.curve_params |} {| CC.curve_constants |} {| bn_ops |} {| f:field_ops |} (out:felem) (b:size_t) : Stack unit
+val fsquare_times_in_place {| cp:S.curve_params |} {| bn_ops |} {| CC.curve_constants |}  {| f:field_ops |} (out:felem) (b:size_t) : Stack unit
   (requires fun h ->
     live h out /\ as_nat h out < S.prime)
   (ensures  fun h0 _ h1 -> modifies (loc out) h0 h1 /\
     as_nat h1 out < S.prime /\
     CC.fmont_as_nat h1 out == SI.fsquare_times (CC.fmont_as_nat h0 out) (v b))
 
-let fsquare_times_in_place {| cp:S.curve_params |} {| CC.curve_constants |} {| bn_ops |} {| f:field_ops |} out b =
+let fsquare_times_in_place {| cp:S.curve_params |} {| bn_ops |} {| CC.curve_constants |}  {| f:field_ops |} out b =
   let h0 = ST.get () in
   SE.exp_pow2_lemma SI.mk_nat_mod_concrete_ops (CC.fmont_as_nat h0 out) (v b);
   BE.lexp_pow2_in_place cp.bn_limbs 0ul mk_pcurve_prime_concrete_ops (null uint64) out b
@@ -92,7 +92,7 @@ let fsquare_times_in_place {| cp:S.curve_params |} {| CC.curve_constants |} {| b
 
 [@(strict_on_arguments [0;1;2;3])]
 inline_for_extraction noextract
-val fsquare_times {| cp:S.curve_params |} {| CC.curve_constants |} {| bn_ops |} {| f:field_ops |} (out a:felem) (b:size_t) : Stack unit
+val fsquare_times {| cp:S.curve_params |} {| bn_ops |} {| CC.curve_constants |}  {| f:field_ops |} (out a:felem) (b:size_t) : Stack unit
   (requires fun h ->
     live h out /\ live h a /\ disjoint out a /\
     as_nat h a < S.prime)
@@ -100,7 +100,7 @@ val fsquare_times {| cp:S.curve_params |} {| CC.curve_constants |} {| bn_ops |} 
     as_nat h1 out < S.prime /\
     CC.fmont_as_nat h1 out == SI.fsquare_times (CC.fmont_as_nat h0 a) (v b))
 
-let fsquare_times {| cp:S.curve_params |} {| CC.curve_constants |} {| bn_ops |} {| f:field_ops |} out a b =
+let fsquare_times {| cp:S.curve_params |} {| bn_ops |} {| CC.curve_constants |}  {| f:field_ops |} out a b =
   let h0 = ST.get () in
   SE.exp_pow2_lemma SI.mk_nat_mod_concrete_ops (CC.fmont_as_nat h0 a) (v b);
   BE.lexp_pow2 cp.bn_limbs 0ul mk_pcurve_prime_concrete_ops (null uint64) a b out
