code/nist-pcurves/Hacl.Impl.PCurves.Group.fsti
@@ -42,29 +42,29 @@ let mk_to_pcurve_comm_monoid {| cp:S.curve_params |} : BE.to_comm_monoid U64 (3u
 
 
 inline_for_extraction noextract
-let point_add_t {| cp:S.curve_params |} {| curve_constants |} {| bn_ops |} {| f:field_ops |} {| curve_inv_sqrt|} = BE.lmul_st U64 (3ul *. cp.bn_limbs) 0ul mk_to_pcurve_comm_monoid
+let point_add_t {| cp:S.curve_params |} {| bn_ops |} {| curve_constants |} {| f:field_ops |} {| curve_inv_sqrt|} = BE.lmul_st U64 (3ul *. cp.bn_limbs) 0ul mk_to_pcurve_comm_monoid
 
 [@(strict_on_arguments [0;1;2;3;4])]
 inline_for_extraction noextract
-val point_add_g {| cp:S.curve_params |} {| curve_constants |} {| bn_ops |} {| f:field_ops |} {| curve_inv_sqrt|} : point_add_t
+val point_add_g {| cp:S.curve_params |} {| bn_ops |} {| curve_constants |} {| f:field_ops |} {| curve_inv_sqrt|} : point_add_t
 
 inline_for_extraction noextract
-let point_double_t {| cp:S.curve_params |} {| curve_constants |} {| bn_ops |} {| f:field_ops |} {| curve_inv_sqrt|} = BE.lsqr_st U64 (3ul *. cp.bn_limbs) 0ul mk_to_pcurve_comm_monoid
-
-[@(strict_on_arguments [0;1;2;3;4])]
-inline_for_extraction noextract
-val point_double_g {| cp:S.curve_params |} {| curve_constants |} {| bn_ops |} {| f:field_ops |} {| curve_inv_sqrt|}: point_double_t
-
-inline_for_extraction noextract
-let point_zero_t {| cp:S.curve_params |} {| curve_constants |} {| bn_ops |} {| f:field_ops |} {| curve_inv_sqrt|} = BE.lone_st U64 (3ul *. cp.bn_limbs) 0ul mk_to_pcurve_comm_monoid
+let point_double_t {| cp:S.curve_params |} {| bn_ops |} {| curve_constants |} {| f:field_ops |} {| curve_inv_sqrt|} = BE.lsqr_st U64 (3ul *. cp.bn_limbs) 0ul mk_to_pcurve_comm_monoid
 
 [@(strict_on_arguments [0;1;2;3;4])]
 inline_for_extraction noextract
-val point_zero_g {| cp:S.curve_params |} {| curve_constants |} {| bn_ops |} {| f:field_ops |} {| curve_inv_sqrt|} : point_zero_t
+val point_double_g {| cp:S.curve_params |} {| bn_ops |} {| curve_constants |} {| f:field_ops |} {| curve_inv_sqrt|}: point_double_t
+
+inline_for_extraction noextract
+let point_zero_t {| cp:S.curve_params |} {| bn_ops |} {| curve_constants |} {| f:field_ops |} {| curve_inv_sqrt|} = BE.lone_st U64 (3ul *. cp.bn_limbs) 0ul mk_to_pcurve_comm_monoid
+
+[@(strict_on_arguments [0;1;2;3;4])]
+inline_for_extraction noextract
+val point_zero_g {| cp:S.curve_params |} {| bn_ops |} {| curve_constants |} {| f:field_ops |} {| curve_inv_sqrt|} : point_zero_t
 
 [@(strict_on_arguments [0;1;2;3;4])]
 inline_for_extraction
-class point_ops {| cp:S.curve_params |} {| curve_constants |} {| bn_ops |} {| field_ops |} {| curve_inv_sqrt|} = {
+class point_ops {| cp:S.curve_params |} {| bn_ops |} {| curve_constants |} {| field_ops |} {| curve_inv_sqrt|} = {
   point_add: point_add_t;
   point_double: point_double_t;
   point_zero: point_zero_t;
@@ -72,7 +72,7 @@ class point_ops {| cp:S.curve_params |} {| curve_constants |} {| bn_ops |} {| fi
 
 [@(strict_on_arguments [0;1;2;3;4;5])]
 inline_for_extraction noextract
-let mk_pcurve_concrete_ops {| S.curve_params |} {| curve_constants |} {| bn_ops |} {| f:field_ops |} {| curve_inv_sqrt|} {| p:point_ops |} : BE.concrete_ops U64 (3ul *. S.bn_limbs) 0ul = {
+let mk_pcurve_concrete_ops {| S.curve_params |} {| bn_ops |} {| curve_constants |} {| f:field_ops |} {| curve_inv_sqrt|} {| p:point_ops |} : BE.concrete_ops U64 (3ul *. S.bn_limbs) 0ul = {
   BE.to = mk_to_pcurve_comm_monoid;
   BE.lone = p.point_zero;
   BE.lmul = p.point_add;
