code/nist-pcurves/Hacl.Impl.PCurves.Point.fst
@@ -29,23 +29,22 @@ let create_point {| cp:S.curve_params |}  =
   create (3ul *. cp.bn_limbs) (u64 0)
 
 
-let make_base_point {| cp:S.curve_params |} {| curve_constants |} p =
+let make_base_point {| cp:S.curve_params |} {| bn_ops |} {| cc:curve_constants |} p =
   let x = getx p in
   let y = gety p in
   let z = getz p in
-  make_g_x x;
-  make_g_y y;
-  make_fone z
+  cc.make_g_x x;
+  cc.make_g_y y;
+  cc.make_fone z
 
 
-[@CInline]
-let make_point_at_inf {| cp:S.curve_params |} {| curve_constants |} p =
+let make_point_at_inf {| cp:S.curve_params |} {| bn_ops |} {| cc:curve_constants |} p =
   let x = getx p in
   let y = gety p in
   let z = getz p in
-  make_fzero x;
-  make_fone y;
-  make_fzero z
+  cc.make_fzero x;
+  cc.make_fone y;
+  cc.make_fzero z
 
 
 ///  Check if a point is a point-at-infinity
@@ -82,7 +81,7 @@ let copy_point res p =
 
 ///  Point conversion between Projective and Affine coordinates representations
 
-let to_aff_point {| cp:S.curve_params |} {| curve_constants |} {| bn_ops |} {| f:field_ops |} {| FI.curve_inv_sqrt|} res p =
+let to_aff_point {| cp:S.curve_params |} {| bn_ops |} {| curve_constants |} {| f:field_ops |} {| FI.curve_inv_sqrt|} res p =
   push_frame ();
   let zinv = create_felem #cp in
   let px = getx p in
@@ -100,7 +99,7 @@ let to_aff_point {| cp:S.curve_params |} {| curve_constants |} {| bn_ops |} {| f
   pop_frame ()
 
 
-let to_aff_point_x {| cp:S.curve_params |} {| curve_constants |} {| bn_ops |} {| f:field_ops |} {| FI.curve_inv_sqrt|} res p =
+let to_aff_point_x {| cp:S.curve_params |} {| bn_ops |} {| curve_constants |} {| f:field_ops |} {| FI.curve_inv_sqrt|} res p =
   push_frame ();
   let zinv = create_felem #cp in
   let px = getx p in
@@ -112,7 +111,7 @@ let to_aff_point_x {| cp:S.curve_params |} {| curve_constants |} {| bn_ops |} {|
   pop_frame ()
 
 
-let to_proj_point {| cp:S.curve_params |} {| curve_constants |} {| bn_ops |} {| f:field_ops |} res p =
+let to_proj_point {| cp:S.curve_params |} {| bn_ops |} {| cc:curve_constants |} {| f:field_ops |} res p =
   let px = aff_getx p in
   let py = aff_gety p in
 
@@ -124,13 +123,13 @@ let to_proj_point {| cp:S.curve_params |} {| curve_constants |} {| bn_ops |} {| 
   SM.lemma_to_from_mont_id (as_nat h0 py);
   f.to_mont rx px;
   f.to_mont ry py;
-  make_fone rz
+  cc.make_fone rz
 
 
 ///  Check if a point is on the curve
 
 inline_for_extraction noextract
-val compute_rp_ec_equation {| cp:S.curve_params |} {| curve_constants |} {| bn_ops |} {| f:field_ops |} :
+val compute_rp_ec_equation {| cp:S.curve_params |} {| bn_ops |} {| cc:curve_constants |} {| f:field_ops |} :
   x:felem -> res:felem -> Stack unit
   (requires fun h ->
     live h x /\ live h res /\ disjoint x res /\
@@ -140,34 +139,34 @@ val compute_rp_ec_equation {| cp:S.curve_params |} {| curve_constants |} {| bn_o
     fmont_as_nat h1 res ==
       S.fadd (S.fadd (S.fmul (S.fmul x x) x) (S.fmul S.a_coeff x)) S.b_coeff))
 
-let compute_rp_ec_equation {| cp:S.curve_params |} {| curve_constants |} {| bn_ops |} {| f:field_ops |} x res =
+let compute_rp_ec_equation {| cp:S.curve_params |} {| bn_ops |} {| cc:curve_constants |} {| f:field_ops |} x res =
   push_frame ();
   let tmp = create_felem #cp in
   fcube res x;
-  make_a_coeff tmp;
+  cc.make_a_coeff tmp;
   f.fmul tmp tmp x;
   f.fadd res tmp res;
-  make_b_coeff tmp;
+  cc.make_b_coeff tmp;
   f.fadd res tmp res;
   pop_frame ()
 
 
 inline_for_extraction noextract
-val is_y_sqr_is_y2_vartime {| cp:S.curve_params |} {| curve_constants |} {| bn_ops |} {| field_ops |} (y2 y:felem) : Stack bool
+val is_y_sqr_is_y2_vartime {| cp:S.curve_params |} {| bn_ops |} {| curve_constants |} {| field_ops |} (y2 y:felem) : Stack bool
   (requires fun h ->
     live h y /\ live h y2 /\ disjoint y y2 /\
     as_nat h y2 < S.prime /\ as_nat h y < S.prime)
   (ensures fun h0 b h1 -> modifies (loc y) h0 h1 /\
     b == (fmont_as_nat h0 y2 = S.fmul (fmont_as_nat h0 y) (fmont_as_nat h0 y)))
 
-let is_y_sqr_is_y2_vartime {| cp:S.curve_params |} {| curve_constants |} {| bn_ops |} {| f:field_ops |} y2 y =
+let is_y_sqr_is_y2_vartime {| cp:S.curve_params |} {| bn_ops |} {| curve_constants |} {| f:field_ops |} y2 y =
   f.fsqr y y; // y = y * y
   let r = feq_mask y y2 in
   Hacl.Bignum.Base.unsafe_bool_of_limb r
 
 
 // y *% y =?= x *% x *% x +% a_coeff *% x +% b_coeff
-let is_on_curve_vartime {| cp:S.curve_params |} {| curve_constants |} {| bn_ops |} {| f:field_ops |} p =
+let is_on_curve_vartime {| cp:S.curve_params |} {| bn_ops |} {| curve_constants |} {| f:field_ops |} p =
   push_frame ();
   let rp = create_felem #cp in
   let tx = create_felem #cp in
@@ -188,13 +187,13 @@ let is_on_curve_vartime {| cp:S.curve_params |} {| curve_constants |} {| bn_ops 
 
 ///  Point load and store functions
 
-let aff_point_store {| cp:S.curve_params |} {| CC.curve_constants |} {| bn_ops |} {| field_ops |} res p =
+let aff_point_store {| cp:S.curve_params |}  {| bn_ops |} {| CC.curve_constants |} {| field_ops |} res p =
   let px = aff_getx p in
   let py = aff_gety p in
   Math.Lemmas.pow2_le_compat (8*cp.bytes) (cp.bits);
   bn2_to_bytes_be res px py
 
-let point_store {| cp:S.curve_params |} {| CC.curve_constants |} {| bn_ops |} {| field_ops |} {| FI.curve_inv_sqrt|} res p =
+let point_store {| cp:S.curve_params |}  {| bn_ops |} {| CC.curve_constants |} {| field_ops |} {| FI.curve_inv_sqrt|} res p =
   push_frame ();
   let aff_p = create_aff_point #cp in
   to_aff_point aff_p p;
@@ -203,14 +202,14 @@ let point_store {| cp:S.curve_params |} {| CC.curve_constants |} {| bn_ops |} {|
 
 
 inline_for_extraction noextract
-val is_xy_valid_vartime {| cp:S.curve_params |} {| curve_constants |} {| bn_ops |} {| field_ops |}:
+val is_xy_valid_vartime {| cp:S.curve_params |} {| bn_ops |} {| curve_constants |} {| field_ops |}:
   p:aff_point -> Stack bool
   (requires fun h -> live h p)
   (ensures fun h0 r h1 -> modifies0 h0 h1 /\
     r == (aff_point_x_as_nat h0 p < S.prime &&
           aff_point_y_as_nat h0 p < S.prime))
 
-let is_xy_valid_vartime {| cp:S.curve_params |} {| curve_constants |} {| bn_ops |} {| f:field_ops |}  p =
+let is_xy_valid_vartime {| cp:S.curve_params |} {| bn_ops |} {| curve_constants |} {| f:field_ops |}  p =
   let px = aff_getx p in
   let py = aff_gety p in
   let lessX = f.bn_is_lt_prime_mask px in
@@ -220,7 +219,7 @@ let is_xy_valid_vartime {| cp:S.curve_params |} {| curve_constants |} {| bn_ops 
   Hacl.Bignum.Base.unsafe_bool_of_limb res
 
 
-let aff_point_load_vartime {| cp:S.curve_params |} {| curve_constants |} {| bn_ops |} {| field_ops |}  p b =
+let aff_point_load_vartime {| cp:S.curve_params |} {| bn_ops |} {| curve_constants |} {| field_ops |}  p b =
   let p_x = sub b 0ul (size cp.bytes) in
   let p_y = sub b (size cp.bytes) (size cp.bytes) in
 
@@ -232,7 +231,7 @@ let aff_point_load_vartime {| cp:S.curve_params |} {| curve_constants |} {| bn_o
   if not is_xy_valid then false
   else is_on_curve_vartime p
 
-let load_point_vartime {| cp:S.curve_params |} {| curve_constants |} {| bn_ops |} {| field_ops |} p b =
+let load_point_vartime {| cp:S.curve_params |} {| bn_ops |} {| curve_constants |} {| field_ops |} p b =
   push_frame ();
   let p_aff = create_aff_point #cp in
   let res = aff_point_load_vartime p_aff b in
@@ -242,7 +241,7 @@ let load_point_vartime {| cp:S.curve_params |} {| curve_constants |} {| bn_ops |
 
 
 inline_for_extraction noextract
-val recover_y_vartime_candidate {| cp:S.curve_params |} {| curve_constants |} {| bn_ops |} {| field_ops |} {| FI.curve_inv_sqrt |} (y x:felem) : Stack bool
+val recover_y_vartime_candidate {| cp:S.curve_params |} {| bn_ops |} {| curve_constants |} {| field_ops |} {| FI.curve_inv_sqrt |} (y x:felem) : Stack bool
   (requires fun h ->
     live h x /\ live h y /\ disjoint x y /\ as_nat h x < S.prime)
   (ensures fun h0 b h1 -> modifies (loc y) h0 h1 /\ as_nat h1 y < S.prime /\
@@ -250,7 +249,7 @@ val recover_y_vartime_candidate {| cp:S.curve_params |} {| curve_constants |} {|
     let y2 = S.(x *% x *% x +% a_coeff *% x +% b_coeff) in
     as_nat h1 y == S.fsqrt y2 /\ (b <==> (S.fmul (as_nat h1 y) (as_nat h1 y) == y2))))
 
-let recover_y_vartime_candidate {| cp:S.curve_params |} {| curve_constants |} {| bn_ops |} {| f:field_ops |} {| FI.curve_inv_sqrt |} y x =
+let recover_y_vartime_candidate {| cp:S.curve_params |} {| bn_ops |} {| curve_constants |} {| f:field_ops |} {| FI.curve_inv_sqrt |} y x =
   push_frame ();
   let y2M = create_felem #cp in
   let xM = create_felem #cp in
@@ -268,7 +267,7 @@ let recover_y_vartime_candidate {| cp:S.curve_params |} {| curve_constants |} {|
 
 
 inline_for_extraction noextract
-val recover_y_vartime {| cp:S.curve_params |} {| curve_constants |} {| bn_ops |} {| field_ops |} {| FI.curve_inv_sqrt |} (y x:felem) (is_odd:bool) : Stack bool
+val recover_y_vartime {| cp:S.curve_params |} {| bn_ops |} {| curve_constants |} {| field_ops |} {| FI.curve_inv_sqrt |} (y x:felem) (is_odd:bool) : Stack bool
   (requires fun h ->
     live h x /\ live h y /\ disjoint x y /\ as_nat h x < S.prime)
   (ensures fun h0 b h1 -> modifies (loc y) h0 h1 /\
@@ -276,16 +275,16 @@ val recover_y_vartime {| cp:S.curve_params |} {| curve_constants |} {| bn_ops |}
     (b ==> (as_nat h1 y < S.prime/\
       as_nat h1 y == Some?.v (S.recover_y (as_nat h0 x) is_odd))))
 
-let recover_y_vartime {| cp:S.curve_params |} {| curve_constants |} {| bn_ops |} {| f:field_ops |} {| FI.curve_inv_sqrt |} y x is_odd =
+let recover_y_vartime {| cp:S.curve_params |} {| bn_ops |} {| curve_constants |} {| f:field_ops |} {| FI.curve_inv_sqrt |} y x is_odd =
   let is_y_valid = recover_y_vartime_candidate y x in
   if not is_y_valid then false
   else begin
     let is_y_odd = bn_is_odd y in
     let is_y_odd = Lib.RawIntTypes.u64_to_UInt64 is_y_odd =. 1uL in
-    f.fnegate_conditional_vartime y (is_y_odd <> is_odd);
+    fnegate_conditional_vartime y (is_y_odd <> is_odd);
     true end
 
-let aff_point_decompress_vartime {| cp:S.curve_params |} {| curve_constants |} {| bn_ops |} {| f:field_ops |} {| FI.curve_inv_sqrt |} x y s =
+let aff_point_decompress_vartime {| cp:S.curve_params |} {| bn_ops |} {| curve_constants |} {| f:field_ops |} {| FI.curve_inv_sqrt |} x y s =
   let s0 = s.(0ul) in
   let s0 = Lib.RawIntTypes.u8_to_UInt8 s0 in
   if not (s0 = 0x02uy || s0 = 0x03uy) then false
