code/nist-pcurves/Hacl.Impl.PCurves.Scalar.fst
@@ -22,11 +22,11 @@ module BM = Hacl.Bignum.Montgomery
 ///  Comparison
 
 
-let bn_is_lt_order_mask_g {| cp:S.curve_params |} {| CC.curve_constants |} {| bn_ops |} f =
+let bn_is_lt_order_mask_g {| cp:S.curve_params |}  {| bn_ops |} {| cc:CC.curve_constants |} f =
   let h0 = ST.get () in
   push_frame ();
   let tmp = create_felem #cp in
-  make_order tmp;
+  cc.make_order tmp;
   let c = bn_sub tmp f tmp in
   assert (if v c = 0 then as_nat h0 f >= S.order else as_nat h0 f < S.order);
   pop_frame ();
@@ -34,7 +34,7 @@ let bn_is_lt_order_mask_g {| cp:S.curve_params |} {| CC.curve_constants |} {| bn
 
 
 
-let bn_is_lt_order_and_gt_zero_mask {| cp:S.curve_params |} {| CC.curve_constants |} {| bn_ops |} f =
+let bn_is_lt_order_and_gt_zero_mask {| cp:S.curve_params |}  {| bn_ops |} {| CC.curve_constants |} f =
   let h0 = ST.get () in
   let is_lt_order = bn_is_lt_order_mask_g f in
   assert (v is_lt_order = (if as_nat h0 f < S.order then ones_v U64 else 0));
@@ -49,7 +49,7 @@ let bn_is_lt_order_and_gt_zero_mask {| cp:S.curve_params |} {| CC.curve_constant
   res
 
 
-let load_qelem_conditional_g {| cp:S.curve_params |} {| CC.curve_constants |} {| bn_ops |} res b =
+let load_qelem_conditional_g {| cp:S.curve_params |}  {| bn_ops |} {| CC.curve_constants |} res b =
   push_frame ();
   bn_from_bytes_be res b;
   let is_b_valid = bn_is_lt_order_and_gt_zero_mask res in
@@ -66,10 +66,11 @@ let load_qelem_conditional_g {| cp:S.curve_params |} {| CC.curve_constants |} {|
 
 ///  Field Arithmetic
 
-val qmod_short_lemma: {| cp:S.curve_params |} -> {| CC.curve_constants |}  -> {| bn_ops |} -> a:nat{a < pow2 (64 * v S.bn_limbs)} ->
+val qmod_short_lemma {| cp:S.curve_params |} {| bn_ops |} {| CC.curve_constants |}:
+  a:nat{a < pow2 (64 * v S.bn_limbs)} ->
   Lemma (let r = if a >= S.order then a - S.order else a in r = a % S.order)
 
-let qmod_short_lemma {| cp:S.curve_params |} {| CC.curve_constants |} {| bn_ops |} a =
+let qmod_short_lemma {| cp:S.curve_params |}  {| bn_ops |} {| CC.curve_constants |} a =
   let r = if a >= S.order then a - S.order else a in
   if a >= S.order then begin
     Math.Lemmas.lemma_mod_sub a S.order 1;
@@ -82,10 +83,10 @@ let qmod_short_lemma {| cp:S.curve_params |} {| CC.curve_constants |} {| bn_ops 
 
 
 
-let qmod_short_g {| cp:S.curve_params |} {| CC.curve_constants |} {| bn_ops |} res x =
+let qmod_short_g {| cp:S.curve_params |}  {| bn_ops |} {| cc:CC.curve_constants |} res x =
   push_frame ();
   let tmp = create_felem #cp in
-  make_order tmp;
+  cc.make_order tmp;
   let h0 = ST.get () in
   let c = bn_sub tmp x tmp in
   bn_cmovznz res c tmp x;
@@ -95,39 +96,19 @@ let qmod_short_g {| cp:S.curve_params |} {| CC.curve_constants |} {| bn_ops |} r
 
 
 
-let qadd_g {| cp:S.curve_params |} {| CC.curve_constants |} {| bn_ops |} res x y =
+let qadd_g {| cp:S.curve_params |}  {| bn_ops |} {| cc:CC.curve_constants |} res x y =
   let h0 = ST.get () in
   push_frame ();
   let n = create_felem #cp in
-  make_order n;
+  cc.make_order n;
   bn_add_mod res n x y;
   let h1 = ST.get () in
   assert (as_nat h1 res == (as_nat h0 x + as_nat h0 y) % S.order);
   SM.qmont_add_lemma (as_nat h0 x) (as_nat h0 y);
   pop_frame ()
 
-inline_for_extraction noextract
-val qmont_reduction: {| cp:S.curve_params |} -> {| CC.curve_constants |}  -> {| bn_ops |} -> res:felem -> x:widefelem -> Stack unit
-  (requires fun h ->
-    live h x /\ live h res /\ disjoint x res /\
-    wide_as_nat h x < S.order * S.order)
-  (ensures fun h0 _ h1 -> modifies (loc res |+| loc x) h0 h1 /\
-    as_nat h1 res == wide_as_nat h0 x * SM.qmont_R_inv % S.order)
 
-
-let qmont_reduction {| cp:S.curve_params |} {| CC.curve_constants |} {| bn_ops |} res x =
-  push_frame ();
-  let n = create_felem #cp in
-  make_order n;
-
-  let h0 = ST.get () in
-  bn_mont_reduction cp.mont_q_mu res x n;
-  SM.bn_qmont_reduction_lemma (as_seq h0 x) (as_seq h0 n);
-  pop_frame ()
-
-
-
-let from_qmont_g {| cp:S.curve_params |} {| CC.curve_constants |} {| bn_ops |} res x =
+let from_qmont_g {| cp:S.curve_params |}  {| bn_ops |} {| cc:CC.curve_constants |} res x =
   push_frame ();
   let tmp = create_widefelem #cp in
   let h0 = ST.get () in
@@ -136,31 +117,31 @@ let from_qmont_g {| cp:S.curve_params |} {| CC.curve_constants |} {| bn_ops |} r
   let h1 = ST.get () in
   assert (wide_as_nat h1 tmp = as_nat h0 x);
   assert_norm (S.order < S.order * S.order);
-  qmont_reduction res tmp;
+  cc.qmont_reduction res tmp;
   pop_frame ()
 
 
 
-let qmul_g {| cp:S.curve_params |} {| CC.curve_constants |} {| bn_ops |} res x y =
+let qmul_g {| cp:S.curve_params |}  {| bn_ops |} {| cc:CC.curve_constants |} res x y =
   push_frame ();
   let tmp = create_widefelem #cp in
   let h0 = ST.get () in
   bn_mul tmp x y;
   let h1 = ST.get () in
   Math.Lemmas.lemma_mult_lt_sqr (as_nat h0 x) (as_nat h0 y) S.order;
-  qmont_reduction res tmp;
+  cc.qmont_reduction res tmp;
   SM.qmont_mul_lemma (as_nat h0 x) (as_nat h0 y);
   pop_frame ()
 
 
 
-let qsqr_g {| cp:S.curve_params |} {| CC.curve_constants |} {| bn_ops |} res x =
+let qsqr_g {| cp:S.curve_params |}  {| bn_ops |} {| cc:CC.curve_constants |} res x =
   push_frame ();
   let tmp = create_widefelem #cp in
   let h0 = ST.get () in
   bn_sqr tmp x;
   let h1 = ST.get () in
   Math.Lemmas.lemma_mult_lt_sqr (as_nat h0 x) (as_nat h0 x) S.order;
-  qmont_reduction res tmp;
+  cc.qmont_reduction res tmp;
   SM.qmont_mul_lemma (as_nat h0 x) (as_nat h0 x);
   pop_frame ()
