code/nist-pcurves/Hacl.Impl.PCurves.Compression.fsti
@@ -27,7 +27,7 @@ val uncompressed_to_raw: {| cp:S.curve_params |} -> pk:lbuffer uint8 (1ul +. 2ul
 
 
 inline_for_extraction noextract
-val compressed_to_raw {| cp:S.curve_params |} {| curve_constants |} {| bn_ops |} {| field_ops |} {| order_ops |} {| curve_inv_sqrt|}:
+val compressed_to_raw {| cp:S.curve_params |} {| bn_ops |} {| curve_constants |} {| field_ops |} {| order_ops |} {| curve_inv_sqrt|}:
   pk:lbuffer uint8 (1ul +. size cp.bytes) ->
   pk_raw:lbuffer uint8 (2ul *. size cp.bytes) -> Stack bool
   (requires fun h -> live h pk /\ live h pk_raw /\ disjoint pk pk_raw)
@@ -37,7 +37,7 @@ val compressed_to_raw {| cp:S.curve_params |} {| curve_constants |} {| bn_ops |}
 
 
 inline_for_extraction noextract
-val raw_to_uncompressed {| cp:S.curve_params |} {| curve_constants |} {| bn_ops |} {| field_ops |} {| order_ops |} {| curve_inv_sqrt|}:
+val raw_to_uncompressed {| cp:S.curve_params |} {| bn_ops |} {| curve_constants |} {| field_ops |} {| order_ops |} {| curve_inv_sqrt|}:
   pk_raw:lbuffer uint8 (2ul *. size cp.bytes) ->
   pk:lbuffer uint8 (1ul +. 2ul *. size cp.bytes) -> Stack unit
   (requires fun h -> live h pk /\ live h pk_raw /\ disjoint pk pk_raw)
@@ -46,7 +46,7 @@ val raw_to_uncompressed {| cp:S.curve_params |} {| curve_constants |} {| bn_ops 
 
 
 inline_for_extraction noextract
-val raw_to_compressed {| cp:S.curve_params |} {| curve_constants |} {| bn_ops |} {| field_ops |} {| order_ops |} {| curve_inv_sqrt|}:
+val raw_to_compressed {| cp:S.curve_params |} {| bn_ops |} {| curve_constants |} {| field_ops |} {| order_ops |} {| curve_inv_sqrt|}:
   pk_raw:lbuffer uint8 (2ul *. size cp.bytes) ->
   pk:lbuffer uint8 (1ul +. size cp.bytes) -> Stack unit
   (requires fun h -> live h pk /\ live h pk_raw /\ disjoint pk pk_raw)
