code/nist-pcurves/Hacl.Impl.PCurves.PointDouble.fsti
@@ -18,7 +18,7 @@ module S = Spec.PCurves
 
 [@(strict_on_arguments [0;1;2;3;4])]
 noextract inline_for_extraction
-val point_double {| cp:S.curve_params |} {| curve_constants |} {| bn_ops |} {| f:field_ops |} {| curve_inv_sqrt|}:
+val point_double {| cp:S.curve_params |} {| bn_ops |} {| curve_constants |} {| f:field_ops |} {| curve_inv_sqrt|}:
   res:point -> p:point -> Stack unit
   (requires fun h ->
     live h p /\ live h res /\ eq_or_disjoint p res /\
